src/Relativization_Examples.thy
@@ -15,22 +15,30 @@ definition test2' :: "i \<Rightarrow> o" where
 definition test3 :: "i" where
   "test3 == {x \<in> 0 . x = x}"
 
+definition test4 :: "o" where
+  "test4 == \<exists>x\<in>1. x = 0"
+
+definition test5 :: "o" where
+  "test5 == \<forall>x\<in>1. x = 0"
+
+definition test6 :: "i \<Rightarrow> i" where
+  "test6(a) = {x \<in> 2 . test2(a)}"
 
 ML\<open>
 structure Ex = struct
-
-  open Relativization
-  fun test_relativ tm ctxt cls_pred db = 
+  val db = Relativization.db
+  fun test_relativ tm ctxt cls_pred db =
   let val pp = Pretty.writeln o Syntax.pretty_term ctxt o Thm.term_of o Thm.cterm_of ctxt
-  in 
+
+  in
    case fastype_of tm of
-      @{typ i} => (pp tm, relativ_tm_frm cls_pred db ctxt tm |> pp)
-    | @{typ o} => (pp tm, relativ_fm cls_pred db ([],ctxt) tm |> pp)
+      @{typ i} => (pp tm, Relativization.relativ_tm_frm cls_pred db ctxt tm |> pp)
+    | @{typ o} => (pp tm, Relativization.relativ_fm cls_pred db ([],ctxt) tm |> pp)
     | ty => raise TYPE ("We can relativize only terms of types i and o",[ty],[tm])
-  end 
+  end
 
   fun relativiz_def ctxt def_name cls_pred db =
-  let 
+  let
     val (_,t,ctxt1) = Utils.thm_concl_tm ctxt (def_name ^ "_def")
     val t = Utils.dest_lhs_def t
   in writeln def_name ; test_relativ t ctxt1 cls_pred db
@@ -38,48 +46,17 @@ structure Ex = struct
 
   fun relativiz_defs ctxt cls_pred db = map (fn d => relativiz_def ctxt d cls_pred db)
 
-  (* relativization db of term constructors *)
-  val ls = [ (@{const Pair}, @{const Relative.pair})
-           , (@{const zero}, @{const Relative.empty})
-           , (@{const succ}, @{const Relative.successor})
-           , (@{const cons}, @{const Relative.is_cons})
-           , (@{const Collect}, @{const Relative.is_Collect})
-           ]
-
-  (* relativization db of relation constructors *)
-  val rs = [ (@{const relation}, @{const Relative.is_relation})
-           , (@{const mem}, @{const mem})
-           , (@{const IFOL.eq(i)}, @{const IFOL.eq(i)})
-           , (@{const Subset}, @{const Relative.subset})
-           ]
-  val db = ls @ rs
-
   (* the class predicate*)
-end
-(*in
-  relativiz_defs @{context} @{term "M :: i \<Rightarrow> o"} db ["test1","test2","test2'","test3"]
-  
-end*)
+end ;
+
+  Ex.relativiz_defs @{context} @{term "M :: i \<Rightarrow> o"} Ex.db
+    ["test4","test5","test1","test2","test2'","test3"]
+
 \<close>
-local_setup\<open>
-  let
-  fun relativized_def ctxt (def_name, thm_ref, cls_pred) =
-  let                                                    
-    val (vars,tm,ctxt1) = Utils.thm_concl_tm ctxt (thm_ref ^ "_def")
-    val (v,t) = tm |> Utils.dest_lhs_def |> Relativization.relativ_tm_frm' cls_pred Ex.db ctxt1
-    val t_vars = Term.add_free_names t []
-    val vs = List.filter (fn (((v,_),_),_)  => Utils.inList v t_vars) vars
-    val vs = [Thm.cterm_of ctxt cls_pred] @ map (op #2) vs @ [Thm.cterm_of ctxt v]
-    val at = List.foldr (fn (var,t') => lambda (Thm.term_of var) t') t vs
-  in
-    Local_Theory.define ((Binding.name def_name, NoSyn), 
-                        ((Binding.name (def_name ^ "_def"), []), at)) #> #2
-  end;
-  in
-    relativized_def @{context} ("is_test", "test1", @{term "M :: i => o"})
-  end
-\<close>
-lemma (in M_trans) test1_abs : "M(a) \<Longrightarrow> M(t) \<Longrightarrow> t = test1(a) \<longleftrightarrow> is_test(M,a,t)"
-  unfolding is_test_def test1_def empty_abs pair_abs by simp
+relativize "test6" "is_test6" "M"
+
+lemma (in M_trivial) test6_abs : "M(a) \<Longrightarrow> M(t) \<Longrightarrow> t = test6(a) \<longleftrightarrow> is_test6(M,a,t)"
+  unfolding test6_def is_test6_def
+  using successor_abs empty_abs by auto
 
 end
