src/Relativization.thy
@@ -1,114 +1,186 @@
 section\<open>Automatic relativization of terms.\<close>
 theory Relativization
   imports "ZF-Constructible.Formula"  "ZF-Constructible.Relative"
+keywords
+  "relativize" :: thy_decl % "ML"
+
 begin
 ML_file\<open>Utils.ml\<close>
+ML\<open>@{term "0\<rightarrow>0"}\<close>
+
 ML\<open>
 structure Relativization  = struct
+  (* For formulas like "t\<in>nat", we don't handle this yet. *)
+  val db_rels_strange = [ (@{const nat} , @{const Relative.finite_ordinal})
+                   , (@{const inj} , @{const Relative.injection})
+                   , (@{const surj} , @{const Relative.surjection})
+                   , (@{const bij} , @{const Relative.bijection})
+                   ]
 
+  (* relativization db of term constructors *)
+  val db_tm_rels = [ (@{const Upair}, @{const Relative.upair})
+           , (@{const Pair}, @{const Relative.pair})
+           , (@{const zero}, @{const Relative.empty})
+           , (@{const succ}, @{const Relative.successor})
+           , (@{const cons}, @{const Relative.is_cons})
+           , (@{const Collect}, @{const Relative.is_Collect})
+           , (@{const Un}, @{const Relative.union})
+           , (@{const Int}, @{const Relative.inter})
+           , (@{const Union}, @{const Relative.big_union})
+           , (@{const Int}, @{const Relative.inter})
+           , (@{const Diff}, @{const Relative.setdiff})
+           , (@{const Image}, @{const Relative.setdiff})
+           , (@{const Sum.sum}, @{const Relative.is_sum})
+           , (@{const Sum.Inl}, @{const Relative.is_Inl})
+           , (@{const Sum.Inr}, @{const Relative.is_Inr})
+           , (@{const domain}, @{const Relative.is_domain})
+           , (@{const range}, @{const Relative.is_range})
+           , (@{const field}, @{const Relative.is_field})
+           , (@{const vimage}, @{const Relative.pre_image})
+           , (@{const apply}, @{const Relative.fun_apply})
+           , (@{const Perm.comp}, @{const Relative.composition})
+           , (@{const Inter}, @{const Relative.big_inter})
+           , (@{const bool_of_o}, @{const Relative.is_bool_of_o})
+           , (@{const Bool.not}, @{const Relative.is_not})
+           , (@{const Bool.and}, @{const Relative.is_and})
+           , (@{const Bool.or}, @{const Relative.is_or})
+           , (@{const List.Nil}, @{const Relative.is_Nil})
+           , (@{const List.Cons}, @{const Relative.is_Cons})
+           , (@{const Relative.is_hd}, @{const Relative.hd'})
+           , (@{const Relative.is_tl}, @{const Relative.tl'})
+           ]
+
+  (* relativization db of relation constructors *)
+  val db_rels = [ (@{const relation}, @{const Relative.is_relation})
+           , (@{const mem}, @{const mem})
+           , (@{const IFOL.eq(i)}, @{const IFOL.eq(i)})
+           , (@{const Subset}, @{const Relative.subset})
+           , (@{const quasinat}, @{const Relative.is_quasinat})
+           , (@{const Transset}, @{const Relative.transitive_set})
+           , (@{const quasinat}, @{const Relative.is_quasinat})
+           , (@{const Ord}, @{const Relative.ordinal})
+           , (@{const Limit}, @{const Relative.limit_ordinal})
+           , (@{const relation}, @{const Relative.is_relation})
+           , (@{const function}, @{const Relative.is_function})
+           , (@{const quasinat}, @{const Relative.is_quasinat})
+           , (@{const Relative.quasilist}, @{const Relative.is_quasilist})
+           ]
+  val db = db_tm_rels @ db_rels
+
+(* t $` u = u $ t*)
 val $` = curry ((op $) o swap)
 infix $`
 
 fun var_i v = Free (v, @{typ i})
+fun var_io v = Free (v, @{typ "i \<Rightarrow> o"})
+fun var_d v = Free (v, dummyT)
 val const_name = #1 o dest_Const
 
 fun lookup f = AList.lookup (fn (x, y) => x = f y)
-fun delete_var v = filter (fn (_,w,_) => w = v)
 val lookup_tm  = AList.lookup (op aconv)
 val update_tm  =  AList.update (op aconv)
 val join_tm = AList.join (op aconv) (fn _ => #1)
-fun lookup_rel c ls =  AList.lookup (op aconv) ls c
+
+(* instantiated with diferent types than lookup_tm *)
+val lookup_rel=  AList.lookup (op aconv)
 
 val conj_ = Utils.binop @{const "IFOL.conj"}
 
-(* We avoid to add a superflous conjunction with True. *)
+(* Conjunction of a list of terms; avoids a superflous conjunction
+with True if the last argument is SOME *)
 fun conjs [] _ = @{term IFOL.True}
   | conjs (f :: []) NONE = f
   | conjs (f :: []) (SOME f') = conj_ f f'
   | conjs (f :: fs) f' = conj_ f (conjs fs f')
 
+(* Produces a relativized existential quantification of the term t *)
+fun rex p t (Free v) = @{const rex} $ p $ lambda (Free v) t
+  | rex _ t (Bound _) = t
+  | rex _ t tm = raise TERM ("rex shouldn't handle this.",[tm,t])
 
-fun exB p t (Free v) = @{const rex} $ p $ lambda (Free v) t
-  | exB _ t (Bound _) = t
-  | exB _ t tm = raise TERM ("exB shouldn't handle this.",[tm,t])
-
-(* constants that do not take the class predicate *)
+(* Constants that do not take the class predicate *)
 val absolute_rels = [ @{const ZF_Base.mem}
                     , @{const IFOL.eq(i)}
                     ]
-fun need_cls_pred c = not (exists (fn t => c aconv t) absolute_rels)
 
-(* Creates the relational term corresponding to a term of type i. If the last 
-  argument is (SOME v) then that variable is not bound by an existential 
+(* Creates the relational term corresponding to a term of type i. If the last
+  argument is (SOME v) then that variable is not bound by an existential
   quantifier.
 *)
-fun close_rel_tm pred tm rs tm_var =
+fun close_rel_tm pred tm tm_var rs =
       let val news = filter (not o (fn x => is_Free x orelse is_Bound x) o #1) rs
           val (vars, tms) = split_list (map (op #2) news)
           val vars = case tm_var of
               SOME w => filter (fn v => not (v = w)) vars
             | NONE => vars
-      in fold (fn v => fn t => exB pred (incr_boundvars 1 t) v) vars (conjs tms tm)
+      in fold (fn v => fn t => rex pred (incr_boundvars 1 t) v) vars (conjs tms tm)
       end
 
-fun relativ_tms _ _ _ ctxt' [] = ([], [], ctxt') 
-  | relativ_tms pred ls rs' ctxt' (u :: us) = 
-      let val (w_u, rs_u, ctxt_u) = relativ_tm pred ls (rs', ctxt') u
-          val (w_us, rs_us, ctxt_us) = relativ_tms pred ls rs_u ctxt_u us
+fun relativ_tms _ _ _ ctxt' [] = ([], [], ctxt')
+  | relativ_tms pred rel_db rs' ctxt' (u :: us) =
+      let val (w_u, rs_u, ctxt_u) = relativ_tm pred rel_db (rs', ctxt') u
+          val (w_us, rs_us, ctxt_us) = relativ_tms pred rel_db rs_u ctxt_u us
       in (w_u :: w_us, join_tm (rs_u , rs_us), ctxt_us)
       end
-and 
+and
     (* The result of the relativization of a term is a triple consisting of
       a. the relativized term (it can be a free or a bound variable but also a Collect)
-      b. a list of (term * (term, term)), taken as a map, which is used to see
+      b. a list of (term * (term, term)), taken as a map, which is used
          to reuse relativization of different occurrences of the same term. The
-         first element is the original term, the second its relativized version, 
+         first element is the original term, the second its relativized version,
          and the last one is the predicate corresponding to it.
       c. the resulting context of creating variables.
     *)
-    relativ_tm pred ls (rs,ctxt) tm = 
-      let 
+    relativ_tm pred rel_db (rs,ctxt) tm =
+      let
       (* relativization of a fully applied constant *)
-      fun relativ_fapp c args abs_args ctxt = case lookup_rel c ls of
-                 SOME p => let 
-                    val (vs, ctxt1) = Variable.variant_fixes [""] ctxt
-                    val v = var_i (hd vs)
+      fun relativ_fapp c args abs_args ctxt = case lookup_rel rel_db c of
+                 SOME p => let
+                    val (v, ctxt1) = Variable.variant_fixes [""] ctxt |>> var_i o hd
                     val r_tm = fold (op $`) (pred :: args @ abs_args @ [v]) p
                     in (v, r_tm, ctxt1)
                     end
-               | NONE   => 
+               | NONE   =>
                   raise TERM ("Constant " ^ const_name c ^ " is not present in the db." , nil)
 
       (* relativization of a partially applied constant *)
       fun relativ_papp tm (t $ u) args abs_args rs' ctxt' = relativ_papp tm t (u :: args) abs_args rs' ctxt'
         | relativ_papp tm (Const c) args abs_args rs' ctxt' =
-            let val (w_ts, rs_ts, ctxt_ts) = relativ_tms pred ls rs' ctxt' args
+            let val (w_ts, rs_ts, ctxt_ts) = relativ_tms pred rel_db rs' ctxt' args
                 val (w_tm, r_tm, ctxt_tm) = relativ_fapp (Const c) w_ts abs_args ctxt_ts
                 val rs_ts' = update_tm (tm, (w_tm, r_tm)) rs_ts
             in  (w_tm, rs_ts', ctxt_tm)
             end
-        | relativ_papp _ t _ _ _ _ = 
-            raise TERM ("Tried to relativize an application with a no-constant in head position",[t])
+        | relativ_papp _ t _ _ _ _ =
+            raise TERM ("Tried to relativize an application with a non-constant in head position",[t])
 
       fun go (Var _) _ _ = raise TERM ("Var: Is this possible?",[])
-        | go (@{const Collect} $ t $ pc) rs ctxt = 
+        | go (@{const Collect} $ t $ pc) rs ctxt =
             relativ_papp tm @{const Collect} [t] [pc] rs ctxt
         | go (tm as Const _) rs ctxt = relativ_papp tm tm [] [] rs ctxt
         | go (tm as t $ u) rs ctxt = relativ_papp tm t [u] [] rs ctxt
         | go tm rs ctxt = (tm, update_tm (tm,(tm,tm)) rs, ctxt)
 
       (* we first check if the term has been already relativized as a variable *)
-      in case lookup_tm rs tm  of
+      in case lookup_tm rs tm of
            NONE => go tm rs ctxt
          | SOME (w, _) => (w, rs, ctxt)
       end
 
-fun relativ_fm pred rel_db (rs,ctxt) fm = 
-  let 
+fun relativ_tm_frm' cls_pred db ctxt tm =
+      let val (w, rs, _) = relativ_tm cls_pred db ([],ctxt) tm
+      in (w, close_rel_tm cls_pred NONE (SOME w) rs)
+      end
+
+fun relativ_tm_frm cls_pred db ctxt = #2 o relativ_tm_frm' cls_pred db ctxt
+
+fun relativ_fm pred rel_db (rs,ctxt) fm =
+  let
 
   (* relativization of a fully applied constant *)
-  fun relativ_fapp c args = case lookup_rel c rel_db of
-         SOME p => let val flag = need_cls_pred c
+  fun relativ_fapp c args = case lookup_rel rel_db c of
+         SOME p => let
+                   val flag = not (exists (curry op aconv c) absolute_rels)
                    in fold (op $`) (if flag then pred :: args else args) p
                    end
        | NONE   => raise TERM ("Constant " ^ const_name c ^ " is not present in the db." , nil)
@@ -118,35 +190,75 @@ fun relativ_fm pred rel_db (rs,ctxt) fm =
      relativizing terms.
    *)
   fun relativ_papp (p $ t) args = relativ_papp p (t :: args)
-    | relativ_papp (Const c) args = 
+    | relativ_papp (Const c) args =
         let val (w_ts, rs_ts, _) = relativ_tms pred rel_db rs ctxt args
             val tm = relativ_fapp (Const c) w_ts
-        in close_rel_tm pred (SOME tm) rs_ts NONE
+        in close_rel_tm pred (SOME tm) NONE rs_ts
         end
     | relativ_papp tm _ =
         raise TERM ("Tried to relativize an application with a no-constant in head position",[tm])
 
+  (* Handling of bounded quantifiers. *)
+  fun bquant quant conn dom pred =
+    let val (v,pred') = Term.dest_abs pred |>> var_i
+    in
+      go (quant $ lambda v (conn $ (@{const mem} $ v $ dom) $ pred'))
+    end
+  and
   (* We could share relativizations of terms occuring inside propositional connectives. *)
-   fun go (@{const IFOL.conj} $ f $ f') = @{const IFOL.conj} $ go f $ go f'
-        | go (@{const IFOL.disj} $ f $ f') = @{const IFOL.disj} $ go f $ go f'
-        | go (@{const IFOL.Not} $ f) = @{const IFOL.Not} $ go f
-        | go (@{const IFOL.iff} $ f $ f') = @{const IFOL.iff} $ go f $ go f'
-        | go (@{const IFOL.imp} $ f $ f') = @{const IFOL.imp} $ go f $ go f'
-        | go (@{const IFOL.All(i)} $ f) = @{const OrdQuant.rall} $ pred $ go f
-        | go (@{const IFOL.Ex(i)} $ f) = @{const OrdQuant.rex} $ pred $ go f
-        | go (Const c) = relativ_fapp (Const c) []
-        | go (p $ t) = relativ_papp p [t]
-        | go (Abs (v,ty,t)) = lambda (Free (v,ty)) (go t)
-        | go t = raise TERM ("Relativization of formulas cannot handle this case.",[t])
-  in  go fm
+      go (@{const IFOL.conj} $ f $ f') = @{const IFOL.conj} $ go f $ go f'
+    | go (@{const IFOL.disj} $ f $ f') = @{const IFOL.disj} $ go f $ go f'
+    | go (@{const IFOL.Not} $ f) = @{const IFOL.Not} $ go f
+    | go (@{const IFOL.iff} $ f $ f') = @{const IFOL.iff} $ go f $ go f'
+    | go (@{const IFOL.imp} $ f $ f') = @{const IFOL.imp} $ go f $ go f'
+    | go (@{const IFOL.All(i)} $ f) = @{const OrdQuant.rall} $ pred $ go f
+    | go (@{const IFOL.Ex(i)} $ f) = @{const OrdQuant.rex} $ pred $ go f
+    | go (@{const Bex} $ f $ Abs p) = bquant @{const Ex(i)} @{const IFOL.conj} f p
+    | go (@{const Ball} $ f $ Abs p) = bquant @{const All(i)} @{const IFOL.imp} f p
+    | go (Const c) = relativ_fapp (Const c) []
+    | go (p $ t) = relativ_papp p [t]
+    | go (Abs body) = body |> Term.dest_abs ||> go |>> var_i |> uncurry lambda
+    | go t = raise TERM ("Relativization of formulas cannot handle this case.",[t])
+  in go fm
   end
 
-  fun relativ_tm_frm' cls_pred db ctxt tm = 
-      let val (w, rs, _) = relativ_tm cls_pred db ([],ctxt) tm
-      in (w, close_rel_tm cls_pred NONE rs (SOME w))
-      end
 
-  fun relativ_tm_frm cls_pred db ctxt = #2 o relativ_tm_frm' cls_pred db ctxt
-end;
+fun relativize_def ctxt cls_pred def_name thm_ref lthy =
+  let
+    val (cls_pred, ctxt1) = Variable.variant_fixes [cls_pred] ctxt |>> var_io o hd
+    val (vars,tm,ctxt1) = Utils.thm_concl_tm ctxt1 (thm_ref ^ "_def")
+    val (v,t) = tm |> #2 o Utils.dest_eq_tms o Utils.dest_trueprop
+                   |> relativ_tm_frm' cls_pred db ctxt1
+    val t_vars = Term.add_free_names t []
+    val vs = List.filter (fn (((v,_),_),_)  => Utils.inList v t_vars) vars
+    val vs = [Thm.cterm_of ctxt cls_pred] @ map (op #2) vs @ [Thm.cterm_of ctxt v]
+    val at = List.foldr (fn (var,t') => lambda (Thm.term_of var) t') t vs
+  in
+   lthy |>
+   Local_Theory.define ((Binding.name def_name, NoSyn),
+                        ((Binding.name (def_name ^ "_def"), []), at)) |>>
+   Pretty.writeln o Syntax.pretty_term ctxt1 o Thm.concl_of o #2 o #2  |> #2
+  end
+end
+\<close>
+
+ML\<open>
+
+local
+  val relativize_parser =
+       Parse.position (Parse.string -- Parse.string -- Parse.string);
+
+  fun in_quote str = "\"" ^ str ^ "\""
+  fun str xs = String.concatWith " " xs
+  val prefix = "Theory.local_setup ((Relativization.relativize_def @{context}"
+  val suffix = "))"
+  val _ =
+     Outer_Syntax.local_theory \<^command_keyword>\<open>relativize\<close> "ML setup for relativizing definitions"
+       (relativize_parser >> (fn (((bndg,thm),pred),p) => ML_Context.expression p (
+        ML_Lex.read (str (prefix :: (map in_quote [pred,thm,bndg]) @ [suffix])))
+        |> Context.proof_map)
+       )
+in
+end
 \<close>
 end
