src/Synthetic_Definition.thy
@@ -1,46 +1,45 @@
 section\<open>Automatic synthesis of formulas\<close>
 theory Synthetic_Definition
-  imports "ZF-Constructible.Formula" Relativization_Examples
-keywords
-  "synthesize" :: thy_decl % "ML"
-and
-  "from_schematic"
+  imports "ZF-Constructible.Formula"
+  keywords
+    "synthesize" :: thy_decl % "ML"
+    and
+    "from_schematic"
 
 begin
 ML_file\<open>Utils.ml\<close>
 
 ML\<open>
-open Utils
 
-fun synthetic_def ctxt (def_name, thm_ref) =
-  let                                                    
-    val (vars,tm,_) = thm_concl_tm ctxt thm_ref 
-    val t = tm |> dest_tp_iff_rhs o dest_trueprop
+fun synthetic_def ctxt def_name thm_ref =
+  let
+    val (vars,tm,_) = Utils.thm_concl_tm ctxt thm_ref
+    val t = tm |> Utils.dest_tp_iff_rhs o Utils.dest_trueprop
     val t_vars = Term.add_free_names t []
-    val vs = List.filter (fn (((v,_),_),_)  => inList v t_vars) vars
+    val vs = List.filter (fn (((v,_),_),_)  => Utils.inList v t_vars) vars
     val at = List.foldr (fn ((_,var),t') => lambda (Thm.term_of var) t') t vs
   in
-    Local_Theory.define ((Binding.name def_name, NoSyn), 
+    Local_Theory.define ((Binding.name def_name, NoSyn),
                         ((Binding.name (def_name ^ "_def"), []), at)) #> snd
-  end;
+  end
 \<close>
 ML\<open>
 
 local
+  val synth_constdecl =
+       Parse.position (Parse.string -- ((Parse.$$$ "from_schematic" |-- Parse.string)));
 
-val synth_constdecl = 
-   Parse.position (Parse.string -- ((Parse.$$$ "from_schematic" |-- Parse.string)));
-
-val _ =  
-  Outer_Syntax.local_theory \<^command_keyword>\<open>synthesize\<close> "ML setup for synthetic definitions" 
- (synth_constdecl >> (fn ((bndg,thm),p) => ML_Context.expression p (
-    ML_Lex.read ("Theory.local_setup ( (synthetic_def @{context} (\"" ^ bndg ^ "\",\"" ^ thm ^ "\")))"))
-  |> Context.proof_map)
- )
+  val _ =
+     Outer_Syntax.local_theory \<^command_keyword>\<open>synthesize\<close> "ML setup for synthetic definitions"
+       (synth_constdecl >> (fn ((bndg,thm),p) => ML_Context.expression p (
+        ML_Lex.read ("Theory.local_setup ( (synthetic_def @{context} \"" ^ bndg ^ "\" \"" ^ thm ^ "\"))"))
+        |> Context.proof_map)
+       )
 in
+
 end
 \<close>
-text\<open>The \<^ML>\<open>synthetic_def\<close> function extracts definitions from 
+text\<open>The \<^ML>\<open>synthetic_def\<close> function extracts definitions from
 schematic goals. A new definition is added to the context. \<close>
 
 (* example of use
@@ -49,7 +48,7 @@ schematic_goal mem_formula_ex :
   shows "nth(m,env) \<in> nth(n,env) \<longleftrightarrow> sats(M,?frm,env)"
   by (insert assms ; (rule sep_rules empty_iff_sats cartprod_iff_sats | simp del:sats_cartprod_fm)+)
 
-synthesize "\<phi>" from_schematic "mem_formula_ex" 
+synthesize "\<phi>" from_schematic "mem_formula_ex"
 
 lemma synth_mem_type : "m \<in> nat \<Longrightarrow> n\<in>nat \<Longrightarrow> \<phi>(n,m) \<in> formula"
   unfolding \<phi>_def by simp
